add toListModel

src/Std/Data/DTreeMap/Internal/WF/Lemmas.lean
@@ -1996,6 +1996,189 @@ theorem WF.filter! {_ : Ord α} {t : Impl α β} {f : (a : α) → β a → Bool
   exact h.filter
 
 /-!
+### interSmaller
+-/
+
+theorem WF.interSmallerFn {_ : Ord α} [TransOrd α] [BEq α] (m₁ : Impl α β) (m₂ : Impl α β)
+    (hm₂ :m₂.WF) (k : α) : (m₁.interSmallerFn ⟨m₂,hm₂.balanced⟩ k).1.WF := by
+  rw [Impl.interSmallerFn]
+  split
+  · exact WF.insert hm₂
+  · exact hm₂
+
+/-- Internal implementation detail of the hash map -/
+def List.interSmallerFn [BEq α] (l sofar : List ((a : α) × β a)) (k : α) : List ((a : α) × β a) :=
+  match List.getEntry? k l with
+  | some kv' => List.insertEntry kv'.1 kv'.2 sofar
+  | none => sofar
+
+theorem List.distinctKeys_interSmallerFn [BEq α] [PartialEquivBEq α]
+    (l sofar : List ((a : α) × β a)) (k : α) (hs : DistinctKeys sofar) :
+    DistinctKeys (interSmallerFn l sofar k) := by
+  rw [interSmallerFn]
+  split
+  · exact hs.insertEntry
+  · exact hs
+
+theorem List.foldl_perm_cong  [BEq α] {init₁ init₂ : List ((a : α) × β a)} {l : List ((a : α) × β a)}
+    {f : List ((a : α) × β a) → ((a : α) × β a) → List ((a : α) × β a)} (h₁ : List.Perm init₁ init₂)
+    (h₂ : ∀ h l₁ l₂, (w : DistinctKeys l₁) → List.Perm l₁ l₂ → List.Perm (f l₁ h) (f l₂ h) ∧ DistinctKeys (f l₁ h))
+    (h₃ : DistinctKeys init₁)
+     : List.Perm (List.foldl f init₁ l) (List.foldl f init₂ l) := by
+  induction l generalizing init₁ init₂
+  case nil =>
+    simp only [List.foldl_nil, h₁]
+  case cons h t ih =>
+    simp only [List.foldl_cons]
+    apply ih
+    · exact (h₂ h init₁ init₂ h₃ h₁).1
+    · exact (h₂ h init₁ init₂ h₃ h₁).2
+
+theorem List.getEntry?_interSmallerFn [BEq α] [PartialEquivBEq α] (l sofar : List ((a : α) × β a)) (k k' : α) :
+    List.getEntry? k' (interSmallerFn l sofar k) =
+      ((List.getEntry? k' l).filter (fun kv => k == kv.1)).or (sofar.getEntry? k') := by
+  rw [interSmallerFn]
+  split
+  · rename_i kv hkv
+    rw [getEntry?_insertEntry]
+    split <;> rename_i hk
+    · have hk' : k == k' := (BEq.trans (BEq.symm (List.beq_of_getEntry?_eq_some hkv)) hk)
+      simp [← List.getEntry?_congr hk', hkv, Option.filter_some, BEq.trans hk' (BEq.symm hk)]
+    · rw [Option.or_eq_right_of_none]
+      apply Option.filter_eq_none_iff.2
+      intro p hp
+      have hp' := List.beq_of_getEntry?_eq_some hp
+      have hkv' := List.beq_of_getEntry?_eq_some hkv
+      exact fun h => hk (BEq.trans hkv' (BEq.trans h hp'))
+  · rename_i hk
+    rw [Option.or_eq_right_of_none]
+    apply Option.filter_eq_none_iff.2
+    intro p hp
+    have := List.beq_of_getEntry?_eq_some hp
+    intro hkp
+    have := BEq.trans hkp this
+    simp [List.getEntry?_congr this, hp] at hk
+
+theorem toListModel_interSmallerFn {_ : Ord α} [TransOrd α] [BEq α] [LawfulBEqOrd α] (m sofar : Impl α β) (h₁ : m.WF) (h₂ : sofar.WF)
+    (l : List ((a : α) × β a))
+    (k : α) (hml : List.Perm (sofar.toListModel) l) :
+    List.Perm (toListModel ((interSmallerFn m ⟨sofar,h₂.balanced⟩ k)).1)
+      (List.interSmallerFn (toListModel m) l k) := by
+  rw [interSmallerFn, List.interSmallerFn]
+  split
+  case h_1 _ val heq =>
+    simp only
+    rw [getEntry?_eq_getEntry?] at heq
+    simp only [heq]
+    apply List.Perm.trans
+    · apply toListModel_insert
+      · exact h₂.ordered
+    · apply insertEntry_of_perm
+      · apply Ordered.distinctKeys h₂.ordered
+      · exact hml
+    · exact h₁.ordered
+  case h_2 heq =>
+    simp only
+    rw [getEntry?_eq_getEntry?] at heq
+    simp only [heq, hml]
+    exact h₁.ordered
+
+/-- Internal implementation detail of the hash map -/
+def List.interSmaller [BEq α] (l₁ l₂ : List ((a : α) × β a)) : List ((a : α) × β a) :=
+  l₂.foldl (fun sofar kv => List.interSmallerFn l₁ sofar kv.1) []
+
+@[simp]
+theorem Option.filter_false {o : Option α} : o.filter (fun _ => false) = none := by
+  cases o <;> simp
+
+theorem Option.filter_or {o : Option α} {p q : α → Bool} : o.filter (fun a => p a || q a) =
+    (o.filter p).or (o.filter q) := by
+  cases o with
+  | none => simp
+  | some a =>
+    simp [Option.filter_some]
+    cases p a <;> cases q a <;> simp
+
+theorem List.getEntry?_interSmaller [BEq α] [PartialEquivBEq α] (l₁ l₂ : List ((a : α) × β a)) (k : α) :
+    List.getEntry? k (interSmaller l₁ l₂) = (List.getEntry? k l₁).filter (fun kv  => containsKey kv.1 l₂) := by
+  rw [interSmaller]
+  suffices ∀ l₃,
+      List.getEntry? k (List.foldl (fun sofar kv => List.interSmallerFn l₁ sofar kv.fst) l₃ l₂) =
+       (Option.filter (fun kv => containsKey kv.fst l₂) (List.getEntry? k l₁)).or (List.getEntry? k l₃) by
+    simpa using this []
+  intro l₃
+  induction l₂ using assoc_induction generalizing l₃ with
+  | nil => simp
+  | cons k v tl ih =>
+    rw [List.foldl_cons, ih]
+    simp only [List.containsKey_cons, Bool.or_comm (k == _), Option.filter_or, Option.or_assoc,
+      List.getEntry?_interSmallerFn]
+
+theorem List.distinctKeys_interSmaller [BEq α] [PartialEquivBEq α] {l₁ l₂ : List ((a : α) × β a)} :
+    DistinctKeys (interSmaller l₁ l₂) := by
+  rw [interSmaller]
+  suffices ∀ l, DistinctKeys l → DistinctKeys (l₂.foldl (fun sofar kv => List.interSmallerFn l₁ sofar kv.1) l) by
+    simpa using this [] (by simp)
+  intro l hl
+  induction l₂ generalizing l with
+  | nil => simpa
+  | cons ht tl ih =>
+    rw [List.foldl_cons]
+    apply ih
+    exact distinctKeys_interSmallerFn _ _ _ hl
+
+theorem List.interSmaller_perm_filter [BEq α] [EquivBEq α] (l₁ l₂ : List ((a : α) × β a)) (h₁ : DistinctKeys l₁) :
+    List.Perm (List.interSmaller l₁ l₂) (l₁.filter (fun kv => containsKey kv.1 l₂)) := by
+  apply List.getEntry?_ext
+  · exact List.distinctKeys_interSmaller
+  · exact h₁.filter (f := fun k v => containsKey k l₂)
+  · intro k'
+    rw [List.getEntry?_filter h₁, List.getEntry?_interSmaller]
+
+theorem toListModel_interSmaller {_ : Ord α} [TransOrd α] [BEq α] [LawfulBEqOrd α]
+    (m₁ : Impl α β) (m₂ : Impl α β) (hm₁ : m₁.WF) :
+    List.Perm (toListModel (m₁.interSmaller m₂))
+      (List.interSmaller (toListModel m₁) (toListModel m₂)) := by
+  rw [interSmaller, foldl_eq_foldl, List.interSmaller]
+  generalize toListModel m₂ = l
+  suffices ∀ m l', (hm : m.WF) → List.Perm (toListModel m) l' →
+      List.Perm (toListModel (List.foldl (fun a b => interSmallerFn m₁ a b.fst) ⟨m, hm.balanced⟩ l).val)
+        (List.foldl (fun sofar kv => List.interSmallerFn (toListModel m₁) sofar kv.fst) l' l) by
+    simpa using this empty [] WF.empty (by simp)
+  intro m l' hm hml'
+  induction l generalizing m l' with
+  | nil => simpa
+  | cons ht tl ih =>
+    rw [List.foldl_cons, List.foldl_cons]
+    exact ih _ _ (by apply WF.interSmallerFn _ _ hm) (toListModel_interSmallerFn _ _ hm₁ hm _ _ hml')
+
+theorem toListModel_inter {_ : Ord α} [TransOrd α] [BEq α] [LawfulBEqOrd α]
+    (m₁ : Impl α β) (m₂ : Impl α β) (hm₁ : m₁.WF) (hm₂ : m₂.WF) :
+    List.Perm (toListModel (m₁.inter m₂ hm₁.balanced)) ((toListModel m₁).filter fun p => containsKey p.1 (toListModel m₂)) := by
+  rw [inter]
+  split
+  · rw [toListModel_filter]
+    conv =>
+      lhs
+      lhs
+      ext e
+      rw [@contains_eq_containsKey α β _ _ _ _ e.fst m₂ hm₂.ordered]
+  · apply List.Perm.trans (toListModel_interSmaller _ _ hm₁) (List.interSmaller_perm_filter _ _ hm₁.ordered.distinctKeys)
+
+theorem inter_eq_inter! [Ord α] {l₁ l₂: Impl α β} {h} :
+    (inter l₁ l₂ h) = inter! l₁ l₂ := by
+  rw [inter, inter!]
+  split
+  · rw [filter_eq_filter!]
+  · rfl
+
+theorem toListModel_inter! {_ : Ord α} [TransOrd α] [BEq α] [LawfulBEqOrd α]
+    (m₁ : Impl α β) (m₂ : Impl α β) (hm₁ : m₁.WF) (hm₂ : m₂.WF) :
+    List.Perm (toListModel (m₁.inter! m₂)) ((toListModel m₁).filter fun p => containsKey p.1 (toListModel m₂)) := by
+  rw [← @inter_eq_inter! _ _ _ _ _ hm₁.balanced]
+  exact toListModel_inter _ _ hm₁ hm₂
+
+/-!
 ### map
 -/
 
